Introduzione dello stato di fallimento. Adattamento lemmi associati e dimostrazioni

MasterThesis/SCORE/Language.lean
@@ -1,49 +1,101 @@
-import Mathlib.Logic.Function.Iterate
+import Mathlib.Data.Prod.Basic
 
 import MasterThesis.Commons
 
 namespace SCORE
 
-def store : Type := ident → List Int
+def store : Type := (ident → List Int) × Bool
+
+def error (s : store) : Prop :=
+  match s with
+  | (_, true ) => False
+  | (_, false) => True
+
+lemma not_error_iff_true {s : store} : ¬error s ↔ ∃ σ, s = (σ, true) := by
+  constructor
+  case mp =>
+    intro
+    match s with
+    | (σ, true ) => exists σ
+    | (σ, false) => simp only [error, not_true_eq_false] at ‹¬error (σ, false)›
+  case mpr =>
+    intro
+    cases ‹∃ σ, s = (σ, true)› with
+    | intro σ => simp only [‹s = (σ, true)›, error, not_false_eq_true]
+
+lemma error_iff_false {s : store} : error s ↔ ∃ σ, s = (σ, false) := by
+  constructor
+  case mp  =>
+    intro
+    match s with
+    | (σ, true ) => simp only [error] at ‹error (σ, true)›
+    | (σ, false) => exists σ
+  case mpr =>
+    intro
+    cases ‹∃ σ, s = (σ, false)› with
+    | intro σ => simp only [‹s = (σ, false)›, error]
 
 namespace store
 
-def emp : store := fun _ => []
+def emp : store := (fun _ => [], true)
 
 def update (x : ident) (l : List Int) (s : store) : store :=
-  fun (y : ident) => if x = y then l else (s y)
+  match s with
+  | (σ, true )  => (fun (y : ident) => if x = y then l else (σ y), true)
+  | (σ, false)  => (σ, false)
 
-notation:100 "[" x:100 " ↦ " l:100 "]" s:100 => update x l s -- Migliorare?
-notation:100 "[" x:100 " ↦ " l:100 "]"       => [x ↦ l] emp -- Migliorare?
+-- TODO: Migliorabile?
+notation:100 "[" x:100 " ↦ " l:100 "]" s:100 => update x l s
+notation:100 "[" x:100 " ↦ " l:100 "]"       => [x ↦ l] emp
 
-#eval (["z" ↦ [3]] ["y" ↦ [2]] ["x" ↦ [1]]) "x"
+#eval (["z" ↦ [3]] ["y" ↦ [2]] ["x" ↦ [1]]).fst "x"
 
 @[simp]
-lemma update_same {s : store} {x y : ident} {l : List Int} : x = y → (store.update x l s) y = l := by
-  intros; simp only [if_pos ‹x = y›, update]
+lemma update_same {s : store} {x y : ident} {l : List Int} : ¬error s → x = y → (store.update x l s).fst y = l := by
+  intros
+  cases (not_error_iff_true.mp ‹¬error s›) with
+  | intro σ => simp only [update, ‹s = (σ, true)›, if_pos ‹x = y›]
 
 @[simp]
-lemma update_other {s : store} {x y : ident} {l : List Int} : x ≠ y → (store.update x l s) y = s y := by
-  intros; simp only [if_neg ‹x ≠ y›, update]
+lemma update_other {s : store} {x y : ident} {l : List Int} : ¬error s → x ≠ y → (store.update x l s).fst y = s.fst y := by
+  intros
+  cases (not_error_iff_true.mp ‹¬error s›) with
+  | intro σ => simp only [update, ‹s = (σ, true)›, if_neg ‹x ≠ y›]
 
-lemma update_shrink {s : store} {x : ident} {l₁ l₂ : List Int} : (store.update x l₂ (store.update x l₁ s)) = store.update x l₂ s := by
-  funext y
-  cases eq_or_ne x y with
-  | inl /- x = y -/ => simp only [update_same ‹x = y›]
-  | inr /- x ≠ y -/ => simp only [update_other ‹x ≠ y›]
-
-lemma update_unchanged {s : store} {x : ident} : s = store.update x (s x) s := by
-  funext y
-  cases eq_or_ne x y with
-  | inl /- x = y -/ => rewrite [‹x = y›]; simp only [update_same]
-  | inr /- x ≠ y -/ => simp only [update_other ‹x ≠ y›]
-
-lemma update_unchanged_cons {s : store} {x : ident} {v : Int} : (s x).head? = some v → s = store.update x (v :: (s x).tail) s := by
+lemma update_shrink {s : store} {x : ident} {l₁ l₂ : List Int} : ¬error s → (store.update x l₂ (store.update x l₁ s)) = store.update x l₂ s := by
   intro
-  have : (v :: (s x).tail) = (s x) := by
-    sorry
-  simp only [‹(v :: (s x).tail) = (s x)›]
-  apply update_unchanged
+  cases (not_error_iff_true.mp ‹¬error s›) with
+  | intro σ =>
+    rw [‹s = (σ, true)›]
+    simp only [update]
+    apply Prod.eq_iff_fst_eq_snd_eq.mpr
+    constructor
+    case intro.left  =>
+      simp only [Prod.fst]
+      funext y
+      cases eq_or_ne x y with
+      | inl /- x = y -/ => simp only [if_pos ‹x = y›]
+      | inr /- x ≠ y -/ => simp only [if_neg ‹x ≠ y›]
+    case intro.right => simp only [Prod.snd]
+
+lemma update_unchanged {s : store} {x : ident} : ¬error s → s = store.update x (s.fst x) s := by
+  intro
+  cases (not_error_iff_true.mp ‹¬error s›) with
+  | intro σ =>
+    rw [‹s = (σ, true)›]
+    simp only [update]
+    apply Prod.eq_iff_fst_eq_snd_eq.mpr
+    constructor
+    case intro.left  =>
+      simp only [Prod.fst]
+      funext y
+      cases eq_or_ne x y with
+      | inl /- x = y -/ => simp only [if_pos ‹x = y›]; rw [‹x = y›]
+      | inr /- x ≠ y -/ => simp only [if_neg ‹x ≠ y›]
+    case intro.right => simp only [Prod.snd]
+
+lemma update_unchanged_cons {s : store} {x : ident} {v : Int} : (s.fst x).head? = some v → s = store.update x (v :: (s.fst x).tail) s := by
+  sorry
 
 end store
 
